% Input your problem and solution below.
% Three dashes on a newline indicate the breaking points.

---

Prove that
\[(x^4+y)(y^4+z)(z^4+x)\ge(x+y^2)(y+z^2)(z+x^2)\]
for all positive real numbers $x$, $y$, $z$ satisfying $xyz\ge1$.

---

Let $L$ and $R$ denote the left- and right-hand expressions. Expanding,
\[L=x^4y^4z^4+\cycsum x^5y^4+\cycsum x^5y+xyz\quad\text{and}\quad R=x^2y^2z^2+\cycsum x^3z^2+\cycsum x^3y+xyz.\]
Subtracting,
\[L-R=\Big(x^4y^4z^4-x^2y^2z^2\Big)+\left(\cycsum x^5y^4-\cycsum x^3z^2\right)+\left(\cycsum x^5z-\cycsum x^3y\right).\]
First, $x^4y^4z^4\ge x^2y^2z^2$ is obvious.

Second, note that
\[\frac{2z^5x^4+x^5y^4}3\ge x^{13/3}y^{4/3}z^{10/3}\ge x^3z^2,\]
and summing, we have $\cycsum x^5y^4\ge\cycsum x^3z^2$.

Third, note that
\[\frac{y^5x+2x^5z}3\ge x^{11/3}y^{5/3}z^{2/3}\ge x^3y,\]
and summing, we have $\cycsum x^5z\ge\cycsum x^3t$.

Hence all the bracketed terms are nonzero, so $L-R\ge0$, as desired.

