% Input your problem and solution below.
% Three dashes on a newline indicate the breaking points.

---

Evaluate \[\sum_{n=1}^\infty\frac1{n^3(n+1)^3}.\]

---

It is well-known that $\sum_{n\ge1}\frac1{n(n+1)}=1$. Consequently, \[\frac{\pi^2}3-1=\sum_{n\ge1}\left(\frac1{n^2}+\frac1{(n+1)^2}\right)=\sum_{n\ge1}\frac{2n(n+1)+1}{n^2(n+1)^2}=2+\sum_{n\ge1}\frac1{n^2(n+1)^2},\]
whence $\sum_{n\ge1}\frac1{n^2(n+1)^2}=\frac13\pi^2-3$. Finally, \[1=\sum_{n\ge1}\left(\frac1{n^3}-\frac1{(n+1)^3}\right)=\sum_{n\ge1}\frac{3n(n+1)+1}{n^3(n+1)^3}=\pi^2-9+\sum_{n\ge1}\frac1{n^3(n+1)^3},\]
and the answer is $\sum_{n\ge1}\frac1{n^3(n+1)^3}=10-\pi^2$.

