% Input your problem and solution below.
% Three dashes on a newline indicate the breaking points.

---

Find all nondecreasing functions $f:\mathbb R_{>0}\to\mathbb R_{>0}$ such that \[f(x^4)+f(x^2)+f(x)+f(1)=x^4+x^2+x+1\]
for all positive real numbers $x$. %https://artofproblemsolving.com/community/c6h1801303p11961334

---

The answer is $f(x)=x$. Substituting $x=1$ into the functional equation gives $f(1)=1$; rewrite the functional equation as \[f(x^4)+f(x^2)+f(x)=x^4+x^2+x.\]
Then $x\mapsto x^8$ gives $f(x^8)+f(x^4)+f(x^2)=x^8+x^4+x^2$, so we have $f(x^8)-x^8=f(x)-x$.
\begin{iclaim*}
    If $x>1$, then $f(x)\ge x$. Similarly if $x<1$, then $f(x)\le x$.
\end{iclaim*}
\begin{proof}
    Assume $x>1$ (thus $f(x)\ge1$) but $f(x)-x=-\veps<0$. Note that for all $k$, we have \[f\left(x^{8^{-k}}\right)-x^{8^{-k}}=f(x)-x=-\veps\implies f\left(x^{8^{-k}}\right)=x^{8^{-k}}-\veps,\]
    which is eventually less than $1$, contradiction.

    An analogous contradiction exists with the assumptions $x<1$ and $f(x)>x$.
\end{proof}

Finally, if $x>1$, then $f(x^4)+f(x^2)+f(x)\ge x^4+x^2+x$, so equality holds and $f(x)=x$. Similarly if $x<1$, then $f(x^4)+f(x^2)+f(x)\le x^4+x^2+x$, so equality holds and $f(x)=x$ again. This completes the proof.

