% Input your problem and solution below.
% Three dashes on a newline indicate the breaking points.

---

If $a$, $b$, $c$ are the sides of a triangle, prove that
\[\frac{\sqrt{b+c-a}}{\sqrt b+\sqrt c-\sqrt a}+\frac{\sqrt{c+a-b}}{\sqrt c+\sqrt a-\sqrt b}+\frac{\sqrt{a+b-c}}{\sqrt a+\sqrt b-\sqrt c}\le3.\]

---

Let $a=(q+r)^2$, $b=(r+p)^2$, $c=(p+q)^2$, so that the desired inequality is
\[\cycsum\frac{\sqrt{p(p+q+r)-qr}}p\le3\sqrt2.\]

Then observe that
\begin{align*}
\left(\cycsum\frac{\sqrt{p(p+q+r)-qr}}p\right)^2
&\le3\cycsum\frac{p(p+q+r)-qr}{p^2}\\
&=3\left(3+\symsum\frac pq-\cycsum\frac{qr}{p^2}\right),
\end{align*}
so it suffices to show
\[3+\cycsum\frac{qr}{p^2}\ge\symsum\frac pq.\]
This is just Schur's inequality on $p^{-2/3}q^{1/3}r^{1/3}$, $p^{1/3}q^{-2/3}r^{1/3}$, $p^{1/3}q^{1/3}r^{-2/3}$:
\begin{align*}
    3\prod\sqrt[3]{\frac{qr}{p^2}}+\cycsum\frac{qr}{p^2}
    &\ge\cycsum\sqrt[3]{\frac{qr}{p^2}}\sqrt[3]{\frac{rp}{q^2}}\left(\sqrt[3]{\frac{qr}{p^2}}+\sqrt[3]{\frac{rp}{q^2}}\right)\\
    &=\cycsum\sqrt[3]{\frac{r^2}{pq}}\left(\frac{q\sqrt[3]r+r\sqrt[3]q}{\sqrt[3]{p^2q^2}}\right)\\
    &=\cycsum\frac{qr+rp}{pq}=\symsum\frac pq.
\end{align*}

