% Input your problem and solution below.
% Three dashes on a newline indicate the breaking points.

---

Compute \[\sum_{k\ge0}\frac{2^k}{5^{2^k}+1}.\]

---

Consider the function \[F(x)&=\sum_{k\ge0}\frac{2^k}{x^{2^k}+1}=\sum_{k\ge0}\sum_{n\ge0}2^k\left(-x^{2^k}\right)^n=\sum_{n\ge0}x^n\sum_{k=0}^{\nu_2(n)}2^k(-1)^{n/2^k}.\]
However \[\sum_{k=0}^{\nu_2(n)}2^k(-1)^{n/2^k}=\left(\sum_{k=0}^{\nu_2(n)-1}2^k\right)-2^{\nu_2(n)}=-1,\]
so $F(x)=\sum_{n\ge0}-x^n=(x-1)^{-1}$, and the answer is $F(5)=1/4$.

---

$1/4$
