% Input your problem and solution below.
% Three dashes on a newline indicate the breaking points.

---

Plugging $x=1,-2$ yields $P(1)=P(-1)=0$. Then, $P(x)=(x-1)(x+1)Q(x)$. Substituting,
\begin{align*}
    x(x-1)(x+2)Q(x+1)&=(x+2)(x-1)(x+1)Q(x)\\
    \implies xQ(x+1)&=(x+1)Q(x).
\end{align*}
Then, $x=0$ gives that $Q(0)=0$, so let $Q(x)=xR(x)$. Substituting, \[x(x+1)R(x+1)=x(x+1)R(x)\implies R(x+1)=R(x)\]
for all $x$, so $R(x)=c$ for some $c$. Then, $P(x)=c(x^3-1)$. We are given that $P(2)^2=P(3)$, so $c=\tfrac23$, and $P(x)=\tfrac23x(x-1)(x+1)$. The answer is $\frac{105}4$, and the requested sum is $105+4=109$.

---

109
