% Input your problem and solution below.
% Three dashes on a newline indicate the breaking points.

---

Let $a>b>c>d$ be positive integers and suppose that \[ac+bd=(b+d+a-c)(b+d-a+c).\]

---

Rearrange as \[ac+bd=(b+d)^2-(a-c)^2\iff b^2+bd+d^2=a^2-ac+c^2.\]
Construct cyclic quadrilateral $WXYZ$ with $WX=a$, $XY=c$, $YZ=b$, $ZW=d$. By Law of Cosines, $\angle WXY=60\dg$ and $\angle YZW=120\dg$. In particular, the aforementioned expression is $WY^2$, so $WY^2\in\mathbb Z$.

By rearrangement $ab+cd>ac+bd>ad+bc$, and by Strong Ptolemy, \[\frac{(ab+cd)(ad+bc)}{ac+bd}=WY^2\in\mathbb Z.\]
This is clearly absurd if $ab+cd$ is prime.

