% Input your problem and solution below.
% Three dashes on a newline indicate the breaking points.

---

Let $\star$ be a binary operation on a set $S$. Suppose that $\star$ is
\begin{enumerate}[label=(\roman*),itemsep=0em]
    \item associative, meaning $a\star(b\star c)=(a\star b)\star c$, and
    \item totally non-commutative, meaning $a\star b\ne b\star a$ whenever $a\ne b$.
\end{enumerate}
Prove that $a\star(b\star c)=a\star c$ for any $a,b,c\in S$.

---

The second condition is better interpreted as follows: if $a\star b=b\star a$, then $a=b$.
\begin{iclaim*}
    We have $a\star a=a$ and $a\star b\star a=a$ for all $a,b\in S$.
\end{iclaim*}
\begin{proof}
    These come from
    \begin{itemize}[itemsep=0em]
        \item $a\star(a\star a)=(a\star a)\star a$ and
        \item $a\star(a\star b\star a)=a\star b\star a=(a\star b\star a)\star b$,
    \end{itemize}
    respectively.
\end{proof}

Finally $(a\star c)\star(a\star b\star c)=a\star b\star c=(a\star b\star c)\star(a\star c)$, and the conclusion follows.

