% Input your problem and solution below.
% Three dashes on a newline indicate the breaking points.

---

Let $m\ge n\ge1$ be integers. Prove that \[\sum_{\substack{a_1+\cdots+a_n=m\\ a_i\ge1}}1^{a_1}2^{a_2}3^{a_3}\cdots n^{a_n}=\sum_{k=1}^n(-1)^{n-k}\binom nkk^m,\]
where the left-hand sum ranges over all $n$-tuples $(a_1,\ldots,a_n)$ of positive integers obeying $a_1+\cdots+a_n=m$.

---

Let \[F(x)=\sum_{m\ge1}\sum_{\substack{a_1+\cdots+a_n=m\\ a_i\ge1}}1^{a_1}2^{a_2}3^{a_3}\cdots n^{a_n}x^m=\frac{n!x^n}{\prod_{k=1}^n(1-kn)}\]
and
\begin{align*}
    G(x)&=\sum_{m\ge1}\sum_{k=1}^n(-1)^{n-k}\binom nkk^mx^m\\
    &=\sum_{k=1}^n(-1)^{n-k}\binom nk\sum_{m\ge1}k^mx^m\\
    &=\sum_{k=1}^n(-1)^{n-k}\binom nk\frac{kx}{1-kx}.
\end{align*}
Denote by $F_0(x)$ and $G_0(x)$ the polynomials obtained by multiplying $F(x)$ and $G(x)$ by $\prod_{k=1}^n(1-kx)$; thus $F_0$ and $G_0$ have degree $n$. We check that $F_0$ and $G_0$ are equal at $n+1$ points, implying the conclusion.

Clearly $F_0(0)=G_0(0)=0$; now we check that for $1\le t\le n$, $F_0(1/t)=G_0(1/t)$ are equal. Indeed,
\begin{align*}
    G_0\left(\frac1t\right)&=(-1)^{n-t}\binom nttx\prod_{k\ne t}\left(1-\frac kt\right)\\
    &=(-1)^{n-t}\binom nt\frac{(-1)^{n-t}(t-1)!(n-t)!}{t^{n-1}}\\
    &=\frac{n!}{t^n}=F_0\left(\frac1t\right),
\end{align*}
and we are done.

